fixed

Phi_System/Fiction_Refinement.thy
@@ -14,7 +14,7 @@ begin
 
 
 
-definition Is_Frame_Proc :: \<open>'ret::VALs proc \<Rightarrow> bool\<close>
+definition Is_Frame_Proc :: \<open>'ret proc \<Rightarrow> bool\<close>
   where \<open>Is_Frame_Proc f \<longleftrightarrow>
     (\<forall>v s s' r. Success v s' \<in> f s \<and> r ## s \<longrightarrow> Success v (r * s') \<in> f (r * s) \<and> r ## s') \<and>
     (\<forall>e s s' r. Abnormal e s' \<in> f s \<and> r ## s \<longrightarrow> Abnormal e (r * s') \<in> f (r * s) \<and> r ## s')\<close>
@@ -38,7 +38,7 @@ lemma
     using prems(1) by blast .
     
 
-definition Transition_of :: \<open>'ret::VALs proc \<Rightarrow> 'ret \<phi>arg + ABNM \<Rightarrow> resource rel\<close>
+definition Transition_of :: \<open>'ret proc \<Rightarrow> 'ret \<phi>arg + ABNM \<Rightarrow> resource rel\<close>
   where \<open>Transition_of f = (\<lambda>x. case x of Inl v \<Rightarrow> { (s,s'). Success v s' \<in> f s \<and> s \<in> RES.SPACE }
                                         | Inr e \<Rightarrow> { (s,s'). Abnormal e s' \<in> f s \<and> s \<in> RES.SPACE } )\<close>
 
@@ -55,28 +55,28 @@ lemma eval_stat_ex:
   by (metis eval_stat.exhaust)
 
 
-definition Transition_of' :: \<open>'ret::VALs proc \<Rightarrow> 'ret eval_stat \<Rightarrow> resource rel\<close>
+definition Transition_of' :: \<open>'ret proc \<Rightarrow> 'ret eval_stat \<Rightarrow> resource rel\<close>
   where \<open>Transition_of' f = (\<lambda>x. (case x of Normal v \<Rightarrow> { (s,s'). Success v s' \<in> f s \<and> s \<in> RES.SPACE }
                                           | Abnm e \<Rightarrow> { (s,s'). Abnormal e s' \<in> f s \<and> s \<in> RES.SPACE }
-                                          | Crash \<Rightarrow> { (s,s'). Invalid \<in> f s \<and> s \<in> RES.SPACE }))\<close>
+                                          | Crash \<Rightarrow> { (s,s'). Invalid \<in> f s \<and> s = s' \<and> s \<in> RES.SPACE }))\<close>
 
 definition Valid_Transition :: \<open>('ret eval_stat \<Rightarrow> 'a rel) \<Rightarrow> bool\<close>
   where \<open>Valid_Transition tr \<longleftrightarrow> tr Crash = {}\<close>
 
 
-definition Transition_of_Success :: \<open>'ret::VALs proc \<Rightarrow> 'ret \<phi>arg \<Rightarrow> resource rel\<close>
+definition Transition_of_Success :: \<open>'ret proc \<Rightarrow> 'ret \<phi>arg \<Rightarrow> resource rel\<close>
   where \<open>Transition_of_Success f = (\<lambda>v. { (s,s'). Success v s' \<in> f s })\<close>
 
 
 
 
-definition Raw_Procedure :: "'ret::VALs proc
+definition Raw_Procedure :: "'ret proc
                         \<Rightarrow> ('ret \<phi>arg \<Rightarrow> resource rel)
                         \<Rightarrow> bool"
     ("\<r>\<a>\<w> \<p>\<r>\<o>\<c> (2_) \<r>\<e>\<f>\<i>\<n>\<e>\<s> _ " [11,11] 10)
   where "Raw_Procedure f S \<longleftrightarrow> (\<forall>x r. f (r * x) \<subseteq> \<S> (\<lambda>v. { r * y | y. (x,y) \<in> S v }) 0)"
 
-definition Fictional_Refine :: "'ret::VALs proc
+definition Fictional_Refine :: "'ret proc
                         \<Rightarrow> ('ret \<phi>arg \<Rightarrow> fiction rel)
                         \<Rightarrow> bool"
   where \<open>Fictional_Refine f S \<longleftrightarrow> (\<forall>x r. f (r * x) \<subseteq> \<S> (\<lambda>v. { r * y | y. (x,y) \<in> S v }) 0)\<close>
@@ -84,13 +84,63 @@ definition Fictional_Refine :: "'ret::VALs proc
 term Domain
 
 definition Fictional_Forward_Simulation :: \<open>'c rel \<Rightarrow> 'a rel \<Rightarrow> ('a::sep_magma_1,'c::sep_magma_1) interp \<Rightarrow> 'a set \<Rightarrow> bool\<close>
-      ("_ \<r>\<e>\<f>\<i>\<n>\<e>\<s> _ \<w>.\<r>.\<t> _ \<i>\<n> _" [11,11,11] 10)
+      ("_/ \<r>\<e>\<f>\<i>\<n>\<e>\<s> _/ \<w>.\<r>.\<t> _/ \<i>\<n> _" [11,11,11] 10)
   where \<open>(F \<r>\<e>\<f>\<i>\<n>\<e>\<s> G \<w>.\<r>.\<t> T \<i>\<n> D) \<longleftrightarrow> (\<forall>x r R. F `` (R * \<I> T (r * x) \<s>\<u>\<b>\<j> r ## x \<and> x \<in> D) \<subseteq> { y'. \<exists>y. y' \<in> R * \<I> T (r * y) \<and> r ## y \<and> (x,y) \<in> G})\<close>
 
 lemma empty_refines_any[simp]:
-  \<open>{} \<r>\<e>\<f>\<i>\<n>\<e>\<s> Any \<w>.\<r>.\<t> I \<i>\<n> AnyD\<close>
+  \<open>{} \<r>\<e>\<f>\<i>\<n>\<e>\<s> Any \<w>.\<r>.\<t> I \<i>\<n> D\<close>
   unfolding Fictional_Forward_Simulation_def
   by simp
+
+lemma refinement_sub_domain:
+  \<open> D' \<subseteq> D
+\<Longrightarrow> A \<r>\<e>\<f>\<i>\<n>\<e>\<s> B \<w>.\<r>.\<t> I \<i>\<n> D
+\<Longrightarrow> A \<r>\<e>\<f>\<i>\<n>\<e>\<s> B \<w>.\<r>.\<t> I \<i>\<n> D'\<close>
+  unfolding Fictional_Forward_Simulation_def
+  by (clarsimp simp add: \<phi>expns subset_iff Image_def Bex_def Id_on_iff, blast)
+
+lemma refinement_sub_fun:
+  \<open> A  \<r>\<e>\<f>\<i>\<n>\<e>\<s> B \<w>.\<r>.\<t> I \<i>\<n> D
+\<Longrightarrow> A' \<subseteq> A
+\<Longrightarrow> A' \<r>\<e>\<f>\<i>\<n>\<e>\<s> B \<w>.\<r>.\<t> I \<i>\<n> D\<close>
+  unfolding Fictional_Forward_Simulation_def
+  by (clarsimp simp add: \<phi>expns subset_iff Image_def Bex_def Id_on_iff; blast)
+
+lemma refinement_sub_fun_right:
+  \<open> A  \<r>\<e>\<f>\<i>\<n>\<e>\<s> B \<w>.\<r>.\<t> I \<i>\<n> D
+\<Longrightarrow> B \<subseteq> B'
+\<Longrightarrow> A \<r>\<e>\<f>\<i>\<n>\<e>\<s> B' \<w>.\<r>.\<t> I \<i>\<n> D\<close>
+  unfolding Fictional_Forward_Simulation_def
+  by (clarsimp simp add: \<phi>expns subset_iff Image_def Bex_def Id_on_iff; blast)
+
+
+lemma refinement_frame:
+  \<open> A \<r>\<e>\<f>\<i>\<n>\<e>\<s> B \<w>.\<r>.\<t> I \<i>\<n> D
+\<Longrightarrow> A \<r>\<e>\<f>\<i>\<n>\<e>\<s> Id_on R * B \<w>.\<r>.\<t> I \<i>\<n> R * D\<close>
+  for B :: \<open>'b::sep_monoid rel\<close>
+  unfolding Fictional_Forward_Simulation_def
+  apply (clarsimp simp add: subset_iff \<phi>expns Image_def Bex_def Id_on_iff)
+  by (smt (z3) sep_disj_multD1 sep_disj_multD2 sep_disj_multI1 sep_disj_multI2 sep_mult_assoc')
+
+(*
+lemma refinement_frame'':
+  \<open> A \<r>\<e>\<f>\<i>\<n>\<e>\<s> B \<w>.\<r>.\<t> I \<i>\<n> D
+\<Longrightarrow> Id_on R * A \<r>\<e>\<f>\<i>\<n>\<e>\<s> Id_on R * B \<w>.\<r>.\<t> I \<i>\<n> R * D\<close>
+  for B :: \<open>'b::sep_monoid rel\<close>
+  unfolding Fictional_Forward_Simulation_def
+  apply (clarsimp simp add: subset_iff \<phi>expns Image_def Bex_def Id_on_iff)
+  subgoal for r R u v u' v' rr a b
+
+lemma refinement_frame':
+  \<open> A \<r>\<e>\<f>\<i>\<n>\<e>\<s> B \<w>.\<r>.\<t> I \<i>\<n> D
+\<Longrightarrow> Id_on UNIV * A = A\<close>
+  unfolding Fictional_Forward_Simulation_def
+  apply (clarsimp simp add: subset_iff \<phi>expns Image_def Bex_def Id_on_iff set_eq_iff; rule)
+   apply clarsimp
+  subgoal for r a b
+
+
+  subgoal for x r R u v rr a' b'
 
 lemma
   \<open>Any \<r>\<e>\<f>\<i>\<n>\<e>\<s> Any \<w>.\<r>.\<t> \<F>_it \<i>\<n> D\<close>
@@ -105,56 +155,162 @@ lemma
   \<open>Any \<r>\<e>\<f>\<i>\<n>\<e>\<s> UNIV \<w>.\<r>.\<t> I\<close>
   unfolding Fictional_Forward_Simulation_def
   apply (clarsimp simp add: subset_iff \<phi>expns Image_def Bex_def Id_on_iff)
-  subgoal for x r R t u v
+  subgoal for x r R t u v *)
 
-
-lemma refinement_frame:
-  \<open> 1 \<in> R
-\<Longrightarrow> A \<r>\<e>\<f>\<i>\<n>\<e>\<s> B \<w>.\<r>.\<t> I
-\<Longrightarrow> A \<r>\<e>\<f>\<i>\<n>\<e>\<s> Id_on R * B \<w>.\<r>.\<t> I\<close>
-  for B :: \<open>'b::sep_monoid rel\<close>
-  unfolding Fictional_Forward_Simulation_def
-  apply (clarsimp simp add: subset_iff \<phi>expns Image_def Bex_def Id_on_iff)
-  by (smt (z3) mult_1_class.mult_1_left mult_1_class.mult_1_right sep_disj_multD2 sep_magma_1_left)
 
 lemma sep_refinement_stepwise:
-  \<open> S1 \<r>\<e>\<f>\<i>\<n>\<e>\<s> S2 \<w>.\<r>.\<t> I1 \<i>\<n> UNIV
+  \<open> S1 \<r>\<e>\<f>\<i>\<n>\<e>\<s> S2 \<w>.\<r>.\<t> I1 \<i>\<n> D
 \<Longrightarrow> S2 \<r>\<e>\<f>\<i>\<n>\<e>\<s> S3 \<w>.\<r>.\<t> I2 \<i>\<n> D'
+\<Longrightarrow> \<forall>r. \<Union> (\<I> I2 ` ({r} * D')) \<subseteq> D
 \<Longrightarrow> S1 \<r>\<e>\<f>\<i>\<n>\<e>\<s> S3 \<w>.\<r>.\<t> (I1 o\<^sub>\<I> I2) \<i>\<n> D'\<close>
-  for S1 :: \<open>'a::sep_monoid rel\<close>
-  and S2 :: \<open>'b::sep_monoid rel\<close>
-  and S3 :: \<open>'c::sep_monoid rel\<close>
   unfolding Fictional_Forward_Simulation_def interp_comp_\<I>
   apply (auto simp add: subset_iff Image_def Bex_def \<phi>expns split_option_all)
   subgoal premises prems for x r R t u v xb
   proof -
-    have \<open>(\<exists>x. (\<exists>u v. x = u * v \<and> u \<in> R \<and> v \<in> \<I> I1 xb \<and> u ## v) \<and> (x, t) \<in> S1)\<close>
-      apply (rule exI[where x=\<open>u * v\<close>], simp add: prems)
-      using prems(6) prems(7) prems(9) by auto
-    note prems(1)[THEN spec[where x=xb],THEN spec[where x=1],THEN spec[where x=\<open>R\<close>],THEN spec[where x=\<open>t\<close>], simplified,
+    thm prems
+    thm prems(1)[THEN spec[where x=xb],THEN spec[where x=1],THEN spec[where x=\<open>R\<close>],THEN spec[where x=\<open>t\<close>]]
+    have \<open>(\<exists>x. (\<exists>u v. x = u * v \<and> u \<in> R \<and> v \<in> \<I> I1 (1 * xb) \<and> u ## v) \<and> 1 ## xb \<and> xb \<in> D \<and> (x, t) \<in> S1)\<close>
+      apply (simp add: prems)
+      using prems(10) prems(3) prems(4) prems(5) prems(6) prems(7) prems(8) prems(9) by blast
+    note prems(1)[THEN spec[where x=xb],THEN spec[where x=1],THEN spec[where x=\<open>R\<close>],THEN spec[where x=\<open>t\<close>],
           THEN mp, OF this]
     then show ?thesis
       apply clarsimp
-      subgoal premises prems2 for y u' v'
+      subgoal premises prems2 for y u'' v''
       proof -
         have \<open>(\<exists>xa. (\<exists>u v. xa = u * v \<and> u \<in> {1} \<and> v \<in> \<I> I2 (r * x) \<and> u ## v) \<and> r ## x \<and> x \<in> D' \<and> (xa, y) \<in> S2)\<close>
-          using prems(3) prems(4) prems(8) prems2(1) by auto
+          by (simp, rule exI[where x=xb], simp add: prems2 prems)
         note prems(2)[THEN spec[where x=x],THEN spec[where x=r],THEN spec[where x=\<open>{1}\<close>], THEN spec[where x=y],
                 THEN mp, OF this]
         then show ?thesis
           apply clarsimp
           using prems2(3) prems2(4) prems2(5) by auto
-      qed
-      .
+      qed .
   qed .
 
-lemma sep_refinement_horizontal_stepwise:
-  \<open> A1 \<r>\<e>\<f>\<i>\<n>\<e>\<s> B1 \<w>.\<r>.\<t> I
-\<Longrightarrow> A2 \<r>\<e>\<f>\<i>\<n>\<e>\<s> B2 \<w>.\<r>.\<t> I
-\<Longrightarrow> A1 O A2 \<r>\<e>\<f>\<i>\<n>\<e>\<s> B1 O B2 \<w>.\<r>.\<t> I\<close>
+lemma sep_refinement_stepwise':
+  \<open> S1 \<r>\<e>\<f>\<i>\<n>\<e>\<s> S2 \<w>.\<r>.\<t> I1 \<i>\<n> D
+\<Longrightarrow> S2' \<r>\<e>\<f>\<i>\<n>\<e>\<s> S3 \<w>.\<r>.\<t> I2 \<i>\<n> D'
+\<Longrightarrow> \<forall>R. \<Union> (\<I> I2 ` (R * D')) \<subseteq> D
+\<Longrightarrow> S2 \<subseteq> S2'
+\<Longrightarrow> S1 \<r>\<e>\<f>\<i>\<n>\<e>\<s> S3 \<w>.\<r>.\<t> (I1 o\<^sub>\<I> I2) \<i>\<n> D'\<close>
+  using refinement_sub_fun sep_refinement_stepwise
+  by metis
+
+
+lemma
+  \<open> A1 \<r>\<e>\<f>\<i>\<n>\<e>\<s> B1 \<w>.\<r>.\<t> I \<i>\<n> D1
+\<Longrightarrow> A2 \<r>\<e>\<f>\<i>\<n>\<e>\<s> B2 \<w>.\<r>.\<t> I \<i>\<n> D2
+\<Longrightarrow> A1 * A2 \<r>\<e>\<f>\<i>\<n>\<e>\<s> B1 * B2 \<w>.\<r>.\<t> I \<i>\<n> D1 * D2\<close>
+  for A1 :: \<open>'a::sep_monoid rel\<close>
   unfolding Fictional_Forward_Simulation_def
   apply (clarsimp simp add: \<phi>expns subset_iff Image_def Bex_def)
-  by (smt (z3) relcomp.relcompI
+  subgoal premises prems for r R u v ux a vx b a' b'
+  proof -
+    thm prems(1)[THEN spec[where x=]]
+    thm prems
+
+
+definition \<open>pairself f = (\<lambda>(x,y). (f x, f y))\<close>
+
+lemma pairself[simp]:
+  \<open>pairself f (x,y) = (f x, f y)\<close>
+  unfolding pairself_def by simp
+
+lemma
+  \<open> \<forall>R. \<Union> (\<I> I2 ` (R * D')) \<subseteq> UNIV * D
+\<Longrightarrow> \<forall>R. \<Union> (\<I> (\<F>_pointwise I2) ` (R * fun_upd 1 k ` D')) \<subseteq> UNIV * fun_upd 1 k ` D\<close>
+  for D :: \<open>'b::sep_monoid set\<close>
+  apply (clarsimp simp add: subset_iff Bex_def image_iff set_mult_expn times_fun)
+  subgoal premises prems for R t u xb
+  proof -
+    thm prems
+    have t1: \<open>u k ## xb\<close>
+      by (metis fun_upd_same prems(4) sep_disj_fun)
+    thm prems
+    thm prems(1)[THEN spec[where x=\<open>{u k}\<close>], THEN spec[where x=\<open>t k\<close>]]
+    have \<open>(\<exists>x. (\<exists>xa. (\<exists>ua v. xa = ua * v \<and> ua \<in> {u k} \<and> v \<in> D' \<and> ua ## v) \<and> x = \<I> I2 xa) \<and> t k \<in> x)\<close>
+      apply simp
+      by (metis prems(2) prems(5) t1)
+    note prems(1)[THEN spec[where x=\<open>{u k}\<close>], THEN spec[where x=\<open>t k\<close>], THEN mp, OF this]
+    then show ?thesis
+      apply clarsimp
+      subgoal premises prems2 for u' v'
+        apply (rule exI[where x=\<open>t(k := u')\<close>], rule exI[where x=\<open>1(k := v')\<close>])
+        by (simp add: fun_eq_iff prems2 sep_disj_fun_def times_fun) .
+  qed .
+
+lemma pointwise_refinement:
+  \<open> Id_on UNIV * A \<r>\<e>\<f>\<i>\<n>\<e>\<s> B \<w>.\<r>.\<t> I \<i>\<n> D
+\<Longrightarrow> Id_on UNIV * pairself (fun_upd 1 k) ` A \<r>\<e>\<f>\<i>\<n>\<e>\<s> pairself (fun_upd 1 k) ` B
+    \<w>.\<r>.\<t> \<F>_pointwise I \<i>\<n> fun_upd 1 k ` D\<close>
+  unfolding Fictional_Forward_Simulation_def
+  apply (clarsimp simp add: \<phi>expns image_iff Image_def subset_iff Bex_def times_fun Id_on_iff)
+  subgoal premises prems for r R u v xb xc a b
+  proof -
+    have t1[simp]: \<open>xc k ## a\<close>
+      by (metis fun_upd_same prems(8) sep_disj_fun)
+    have t2[simp]: \<open>xc k ## b\<close>
+      by (metis fun_upd_same prems(9) sep_disj_fun)
+    have \<open>(\<exists>x. (\<exists>ua v. x = ua * v \<and> ua \<in> {u k} \<and> v \<in> \<I> I (r k * xb) \<and> ua ## v) \<and>
+     r k ## xb \<and>
+     xb \<in> D \<and> (\<exists>a ba aa. x = a * aa \<and> (\<exists>bb. xc k * b = ba * bb \<and> a = ba \<and> (aa, bb) \<in> A \<and> a ## aa \<and> ba ## bb)))\<close>
+      apply (simp add: prems)
+      by (smt (verit, del_insts) fun_upd_same prems(10) prems(2) prems(5) prems(6) prems(7) sep_disj_fun_def t1 t2 times_fun)
+    note prems(1)[THEN spec[where x=xb], THEN spec[where x=\<open>r k\<close>], THEN spec[where x=\<open>{u k}\<close>, THEN spec[where x=\<open>xc k * b\<close>]],
+          THEN mp, OF this]
+    then show ?thesis
+      apply clarsimp
+      subgoal premises prems2 for y v'
+      proof -
+        thm prems
+        thm prems2
+        have t4: \<open>u ## v(k := v')\<close>
+          by (clarsimp simp add: sep_disj_fun_def prems2 prems(7)) (simp add: prems(7))
+        have t3: \<open>xc * 1(k := b) = u * v(k := v')\<close>
+          apply (clarsimp simp add: fun_eq_iff times_fun prems2)
+          by (metis (no_types, opaque_lifting) fun_upd_other mult_1_class.mult_1_right prems(5) times_fun_def)
+        show ?thesis
+        apply (rule exI[where x=\<open>1(k := y)\<close>]; simp add: prems prems2; rule)
+          apply (smt (verit, ccfv_threshold) fun_split_1 fun_upd_other fun_upd_same prems(3) prems(6) prems2(4) t3 t4 times_fun)
+          by (metis fun_sep_disj_1_fupdt(1) fun_upd_triv prems2(1) prems2(2))
+      qed .
+  qed .
+
+
+lemma sep_refinement_horizontal_stepwise:
+  \<open> A1 \<r>\<e>\<f>\<i>\<n>\<e>\<s> B1 \<w>.\<r>.\<t> I \<i>\<n> D
+\<Longrightarrow> A2 \<r>\<e>\<f>\<i>\<n>\<e>\<s> B2 \<w>.\<r>.\<t> I \<i>\<n> D'
+\<Longrightarrow> (B1 `` D \<subseteq> D')
+\<Longrightarrow> A1 O A2 \<r>\<e>\<f>\<i>\<n>\<e>\<s> B1 O B2 \<w>.\<r>.\<t> I \<i>\<n> D\<close>
+  unfolding Fictional_Forward_Simulation_def
+  apply (clarsimp simp add: \<phi>expns subset_iff Image_def Bex_def)
+  subgoal premises prems for x r R u v y z
+  proof -
+    have \<open>(\<exists>xa. (\<exists>u v. xa = u * v \<and> u \<in> R \<and> v \<in> \<I> I (r * x) \<and> u ## v) \<and> r ## x \<and> x \<in> D \<and> (xa, y) \<in> A1)\<close>
+      using prems(10) prems(4) prems(5) prems(6) prems(8) prems(9) by blast
+    note prems(1)[THEN spec[where x=x], THEN spec[where x=r], THEN spec[where x=R], THEN spec[where x=y],
+          THEN mp, OF this]
+    then show ?thesis
+      apply clarsimp
+      subgoal premises prems2 for y' u' v'
+      proof -
+        have \<open>(\<exists>x. (\<exists>u v. x = u * v \<and> u \<in> R \<and> v \<in> \<I> I (r * y') \<and> u ## v) \<and> r ## y' \<and> y' \<in> D' \<and> (x, z) \<in> A2)\<close>
+          using prems(3) prems(5) prems(7) prems2(1) prems2(2) prems2(3) prems2(4) prems2(5) prems2(6) by blast
+        note prems(2)[THEN spec[where x=y'], THEN spec[where x=r], THEN spec[where x=R], THEN spec[where x=z],
+          THEN mp, OF this]
+        then show ?thesis
+          apply clarsimp
+          using prems2(2) by blast
+      qed .
+  qed .
+
+
+context perm_ins_homo begin
+
+
+
+end
 
 
 context basic_fiction begin
@@ -174,38 +330,38 @@ lemma
     thm prems(4)[THEN spec[where x=v], THEN spec[where x=x], THEN spec[where x=\<open>get r\<close>], THEN spec[where x=\<open>{u}\<close>], THEN spec[where x=\<open>y'\<close>]]
   proof -
     have [simp]: \<open>R.clean y' \<in> R.SPACE\<close>
-      by (metis (no_types, lifting) R.\<r>_valid_split R.inj.homo_sep_mult_axioms Valid_Proc_def homo_sep_mult.homo_mult prems(1) prems(10) prems(14) prems(15) prems(16) prems(9) times_fupdt_1_apply_sep times_fupdt_1_fupdt_1_sep)
+      by (metis R.\<r>_valid_split Valid_Proc_def fun_upd_same fun_upd_upd prems(1) prems(11) prems(13) prems(14) prems(16) prems(17) prems(9) resource_space.SPACE_1 resource_space.SPACE_mult_homo)
     have t2: \<open>(\<exists>xa. (\<exists>ua v. xa = ua * v \<and> ua \<in> {u} \<and> (\<exists>xa. xa \<in> \<I> I (get r * x) \<and> v = R.mk xa) \<and> ua ## v) \<and>
-      get r ## x \<and> x \<in> D \<and> Success v y' \<in> f xa \<and> R.clean xa \<in> R.SPACE \<and> (\<exists>m. xa R.name = R.inject m \<and> m \<in>\<^sub>S R.domain))\<close>
+      get r ## x \<and> x \<in> D \<and> Success v y' \<in> f xa \<and> R.clean xa \<in> R.SPACE \<and> (\<exists>m. xa R.name = R.inject m \<and> m \<in>\<^sub>S\<^sub>H R.domain))\<close>
       apply (rule exI[where x=\<open>(u * R.mk y)\<close>], simp add: prems R.inj.homo_mult[symmetric] )
-      using prems(12) prems(13) by blast
+      using prems(11) prems(12) by blast
     note prems(4)[THEN spec[where x=v], THEN spec[where x=x], THEN spec[where x=\<open>get r\<close>], THEN spec[where x=\<open>{u}\<close>], THEN spec[where x=\<open>y'\<close>],
             THEN mp, OF this]
     then show ?thesis
     apply clarsimp
     subgoal for yy ya
       apply (rule exI[where x=yy], clarsimp simp add: inj.homo_mult[symmetric] prems prj.homo_mult, rule)
-      apply (metis R.resource_kind_axioms Valid_Proc_def prems(1) prems(15) resource_kind.\<r>_valid_split t2 times_fupdt_1_apply_sep)
-      using prems(11) by blast .
+      apply (metis R.resource_kind_axioms Valid_Proc_def prems(1) prems(14) resource_kind.\<r>_valid_split t2 times_fupdt_1_apply_sep)
+      using prems(10) by blast .
 qed
   subgoal premises prems for r u y v y' rr
   proof -
     thm prems(5)[THEN spec[where x=v], THEN spec[where x=x], THEN spec[where x=\<open>get r\<close>], THEN spec[where x=\<open>{u}\<close>], THEN spec[where x=\<open>y'\<close>]]
     have [simp]: \<open>R.clean y' \<in> R.SPACE\<close>
-      by (metis R.\<r>_valid_split R.inj.homo_mult Valid_Proc_def prems(1) prems(10) prems(14) prems(15) prems(16) prems(9) times_fupdt_1_apply_sep times_fupdt_1_fupdt_1_sep)
+      by (metis R.\<r>_valid_split Valid_Proc_def fun_upd_same fun_upd_upd prems(1) prems(11) prems(13) prems(14) prems(16) prems(17) prems(9) resource_space.SPACE_1 resource_space.SPACE_mult_homo)
     have t2: \<open>(\<exists>xa. (\<exists>ua v. xa = ua * v \<and> ua \<in> {u} \<and> (\<exists>xa. xa \<in> \<I> I (get r * x) \<and> v = R.mk xa) \<and> ua ## v) \<and>
-      get r ## x \<and> x \<in> D \<and> Abnormal v y' \<in> f xa \<and> R.clean xa \<in> R.SPACE \<and> (\<exists>m. xa R.name = R.inject m \<and> m \<in>\<^sub>S R.domain))\<close>
-      by (metis (no_types, lifting) R.inj.homo_mult fiction_kind.sep_disj_get_name_eq fiction_kind_axioms insert_iff prems(10) prems(12) prems(13) prems(14) prems(15) prems(16) prems(3) prems(7) prems(8) prems(9) times_fupdt_1_apply_sep times_fupdt_1_fupdt_1_sep)
+      get r ## x \<and> x \<in> D \<and> Abnormal v y' \<in> f xa \<and> R.clean xa \<in> R.SPACE \<and> (\<exists>m. xa R.name = R.inject m \<and> m \<in>\<^sub>S\<^sub>H R.domain))\<close>
+      by (metis (no_types, lifting) R.inj.homo_mult fiction_kind.sep_disj_get_name_eq fiction_kind_axioms insert_iff mult_in_sep_homo_set prems(11) prems(12) prems(13) prems(14) prems(15) prems(16) prems(17) prems(3) prems(7) prems(8) prems(9) times_fupdt_1_apply_sep times_fupdt_1_fupdt_1_sep)
     note prems(5)[THEN spec[where x=v], THEN spec[where x=x], THEN spec[where x=\<open>get r\<close>], THEN spec[where x=\<open>{u}\<close>], THEN spec[where x=\<open>y'\<close>],
             THEN mp, OF this]
     then show ?thesis
       apply clarsimp
       subgoal for yy ya
         apply (rule exI[where x=yy], clarsimp simp add: inj.homo_mult[symmetric] prems prj.homo_mult, rule)
-        apply (metis R.resource_kind_axioms Valid_Proc_def prems(1) prems(15) resource_kind.\<r>_valid_split t2 times_fupdt_1_apply_sep)
-        using prems(11) by blast .
+        apply (metis R.\<r>_valid_split Valid_Proc_def prems(1) prems(14) t2 times_fupdt_1_apply_sep)
+        using prems(10) by blast .
   qed
-  by (metis (mono_tags, lifting) R.inj.homo_mult sep_disj_get_name times_fupdt_1_apply_sep times_fupdt_1_fupdt_1_sep)
+  by (metis (no_types, lifting) R.inj.homo_mult mult_in_sep_homo_set sep_disj_get_name times_fupdt_1_apply_sep times_fupdt_1_fupdt_1_sep)
 
 end
 
@@ -221,85 +377,228 @@ lemma GTS_iff[iff]:
 
 
 
+context partial_map_resource2 begin
 
+lemma
+  \<open>{(x,y). x \<in> SPACE \<and> y = updt (map_fun_at (map_fun_at (\<lambda>_. u) k2) k) x}
+\<r>\<e>\<f>\<i>\<n>\<e>\<s> {(1(k := 1(k2 \<mapsto> any)), 1(k := 1(k2 := u))) | any. True}
+\<w>.\<r>.\<t> basic_fiction \<i>\<n> {(1(k := 1(k2 \<mapsto> any))) | any. True}\<close>
+unfolding Fictional_Forward_Simulation_def
+  apply (clarsimp simp add: basic_fiction_\<I> \<phi>expns prj.homo_mult times_fun_upd sep_disj_partial_map_upd
+        nonsepable_semigroup_sepdisj_fun SPACE_mult_homo \<r>_valid_split'
+        times_fun inj.homo_mult[symmetric] inject_wand_homo)
+  apply rule
+  subgoal premises prems for r R u' any a
+    apply (rule exI[where x=u']; simp add: prems; rule)
+  proof -
+    have [simp]: \<open>(r * a) k k2 = None\<close>
+      by (smt (verit, best) fun_upd_same prems(3) prems(7) sep_disj_fun_def sep_disj_multD1 sep_disj_multI1 sep_disj_partial_map_some_none sep_mult_commute)
+    then have [simp]:
+        \<open>map_fun_at (map_fun_at (\<lambda>_. u) k2) k (r * (a * 1(k := 1(k2 \<mapsto> any))))
+            = (r * a) * 1(k := 1(k2 := u))\<close>
+        unfolding map_fun_at_def fun_eq_iff times_fun_def
+        by simp
+    have t1[simp]: \<open>clean u' * mk a = u'\<close>
+      by (metis fun_split_1 prems(6))
+    show \<open>clean u' * mk (map_fun_at (map_fun_at (\<lambda>_. u) k2) k (r * (a * 1(k := 1(k2 \<mapsto> any))))) = u' * mk (r * 1(k := 1(k2 := u)))\<close>
+        apply simp
+      by (smt (verit, del_insts) fun_sep_disj_1_fupdt(1) fun_upd_triv inj.homo_mult inj.sep_disj_homo inject_assoc_homo nonsepable_semigroup_sepdisj_fun prems(3) prems(6) prems(7) sep_disj_multD1 sep_disj_multI1 sep_mult_commute sep_space_entry.times_fun_upd sep_space_entry_axioms times_fupdt_1_apply_sep)
+    show \<open>u' ## mk (r * 1(k := 1(k2 := u)))\<close>
+      by (metis fun_sep_disj_1_fupdt(1) fun_upd_triv inj.sep_disj_homo nonsepable_semigroup_sepdisj_fun prems(3) prems(6) prems(7) sep_disj_multD1 sep_disj_multI1 sep_disj_multI2)
+  qed
+  by (metis fun_sep_disj_1_fupdt(1) fun_upd_triv nonsepable_semigroup_sepdisj_fun)
+
+lemma
+  \<open>Transition_of' (\<phi>R_set_res (map_fun_at (map_fun_at (\<lambda>_. u) k2) k)) ret
+= {(x,y). x \<in> SPACE \<and> y = updt (map_fun_at (map_fun_at (\<lambda>_. u) k2) k) x \<and> ret = Normal \<phi>V_none}\<close>
+  unfolding Transition_of'_def \<phi>R_set_res_def
+  by (cases ret; clarsimp simp add: set_eq_iff \<phi>V_none_def; rule; clarsimp)
+
+lemma
+  \<open>Transition_of' (\<phi>R_set_res (map_fun_at (map_fun_at (\<lambda>_. u) k2) k)) ret
+    \<r>\<e>\<f>\<i>\<n>\<e>\<s> {(x,y). x \<in> SPACE \<and> y = updt (map_fun_at (map_fun_at (\<lambda>_. u) k2) k) x \<and> ret = Normal \<phi>V_none}
+    \<w>.\<r>.\<t> \<F>_it \<i>\<n> { 1(Res #= 1(k := 1(k2 \<mapsto> any))) | any. True }\<close>
+  unfolding Transition_of'_def \<phi>R_set_res_def
+  apply (cases ret; clarsimp simp add: Fictional_Forward_Simulation_def subset_iff Image_iff
+        \<phi>expns Bex_def SPACE_mult_homo)
+  subgoal premises prems for r R u' any
+  proof -
+    thm prems
+    have t1[simp]: \<open>r ## (u' * mk (1(k := 1(k2 \<mapsto> any))))\<close>
+      by (simp add: prems(2) prems(4) sep_disj_commuteI sep_disj_multI1 sep_mult_commute)
+    have t11[simp]: \<open>u' ## mk (1(k := 1(k2 \<mapsto> any)))\<close>
+      using prems(2) prems(4) sep_disj_commuteI sep_disj_multD2 by blast 
+    have t12[simp]: \<open>r * u' ## mk (1(k := 1(k2 \<mapsto> any)))\<close>
+      by (simp add: sep_disj_multI1)
+    have t12'[simp]: \<open>get (r * u') ## (1(k := 1(k2 \<mapsto> any)))\<close>
+      using sep_disj_get_name t12 by blast
+    have txx[simp]: \<open>get (r * u') k k2 = None\<close>
+      by (metis (mono_tags, opaque_lifting) fun_sep_disj_imply_v fun_upd_triv sep_disj_option_nonsepable(1) t12')
+    have t01[simp]: \<open>r * (u' * mk (1(k := 1(k2 := xx)))) = (r * u') * mk (1(k := 1(k2 := xx)))\<close> for xx
+      by (metis (mono_tags, lifting) SPACE_mult_homo fun_sep_disj_1_fupdt(1) fun_upd_triv inj.sep_disj_homo inj_prj_in_SPACE nonsepable_semigroup_sepdisj_fun prems(5) sep_disj_multD1 sep_mult_assoc t1 t11 t12')
+    have t02[simp]: \<open>u' * (r * mk (1(k := 1(k2 := xx)))) = (r * u') * mk (1(k := 1(k2 := xx)))\<close> for xx
+      by (smt (z3) SPACE_mult_homo fun_sep_disj_1_fupdt(1) fun_upd_triv inj.sep_disj_homo inj_prj_in_SPACE nonsepable_semigroup_sepdisj_fun prems(2) prems(4) prems(5) sep_disj_multD1 sep_disj_multI1 sep_mult_assoc sep_mult_commute t1 t11 times_fun)
+    have t5[simp]: \<open>map_fun_at (map_fun_at (\<lambda>_. u) k2) k (1(k := 1(k2 \<mapsto> any))) = (1(k := 1(k2 := u)))\<close>
+      by (simp add: map_fun_at_def fun_eq_iff)
+    have t4[simp]: \<open>map_fun_at (map_fun_at (\<lambda>_. u) k2) k (get (r * u') * 1(k := 1(k2 \<mapsto> any))) = get (r * u') * 1(k := 1(k2 := u))\<close>
+      unfolding map_fun_at_def fun_eq_iff
+      by simp
+    have t6[simp]: \<open>project ((r * u') name * inject (1(k := 1(k2 \<mapsto> any)))) = get (r * u') * 1(k := 1(k2 \<mapsto> any))\<close>
+      by (simp add: prj.homo_mult)
+
+    show ?thesis
+      apply (rule, rule exI[where x=u'], simp add: prems, rule)
+      apply (smt (verit, ccfv_threshold) SPACE_mult_homo fun_sep_disj_1_fupdt(1) fun_upd_triv inj.homo_mult inj_prj_in_SPACE nonsepable_semigroup_sepdisj_fun prems(5) sep_space_entry.times_fun_upd sep_space_entry_axioms t01 t12 t12' times_fupdt_1_apply_sep)
+       apply (smt (verit, del_insts) SPACE_mult_homo fun_sep_disj_1_fupdt(1) fun_upd_triv inj.sep_disj_homo_semi inj_prj_in_SPACE nonsepable_semigroup_sepdisj_fun prems(2) prems(4) prems(5) sep_disj_multD1 sep_disj_multI2 sep_mult_commute t1 t11 t12')
+      apply (simp add: \<phi>V_none_def; rule)
+      apply (metis (mono_tags, lifting) SPACE_mult_homo fun_sep_disj_1_fupdt(1) fun_upd_triv inj.sep_disj_homo inj_prj_in_SPACE nonsepable_semigroup_sepdisj_fun prems(2) prems(5) t1)
+      using SPACE_mult_homo prems(5) by force      
+  qed .
+
+end
+
+context resource begin
+
+lemma
+  \<open> Transition_of' (\<phi>R_get_res F) ret = {(s,s'). (s,s') \<in> Transition_of' (F (get s)) ret}\<close>
+  unfolding Transition_of'_def \<phi>R_get_res_def
+  by (cases ret; clarsimp simp add: set_eq_iff)
+
+lemma \<phi>R_get_res_transition:
+  \<open> (\<And>res. Transition_of' (F res) ret \<subseteq> Id_on (UNIV \<s>\<u>\<b>\<j> res \<in> UNIV * P ret))
+\<Longrightarrow> Transition_of' (\<phi>R_get_res F) ret \<subseteq> Id_on SPACE * Id_on (mk ` P ret)\<close>
+  unfolding Transition_of'_def \<phi>R_get_res_def
+  apply (cases ret; clarsimp simp add: set_eq_iff Id_on_iff subset_iff Subjection_expn image_iff
+            Bex_def set_mult_expn)
+  apply (smt (verit, ccfv_threshold) SPACE_mult_homo fun_sep_disj_1_fupdt(1) fun_split_1 inj_prj_in_SPACE mk_homo_mult sep_disj_clean sep_disj_mk sep_mult_assoc' times_fun_upd
+  apply (smt (verit) SPACE_mult_homo fun_split_1 inj_prj_in_SPACE mk_homo_mult sep_disj_clean sep_disj_mk sep_disj_multI1 sep_mult_assoc'
+  by (smt (z3) SPACE_mult_homo fun_split_1 inj_prj_in_SPACE mk_homo_mult sep_disj_clean sep_disj_mk sep_disj_multI1 sep_mult_assoc'
+  
+(*
+  term apply (metis \<r>_valid_split fun_split_1 proj_inj sep_disj_clean)
+  apply (metis \<r>_valid_split fun_split_1 proj_inj sep_disj_clean)
+  by (metis sep_disj_clean) *)
+
+end
 
 context partial_map_resource begin
 
-term \<open>{(x,y). y = updt (\<lambda>f. f(k := u)) x}\<close>
+lemma
+  \<open>(\<And>v. Transition_of' (F v) ret \<subseteq> Id_on (UNIV \<s>\<u>\<b>\<j> v \<in> P ret))
+\<Longrightarrow> Transition_of' (case res k of Some v \<Rightarrow> F v | _ \<Rightarrow> (\<lambda>_. {Invalid})) ret
+      \<subseteq> Id_on (UNIV \<s>\<u>\<b>\<j> res \<in> UNIV * (\<lambda>v. 1(k \<mapsto> v)) ` P ret)\<close>
+  unfolding Transition_of'_def
+  apply (cases ret; clarsimp simp add: Id_on_iff subset_iff Subjection_expn set_mult_expn
+                      image_iff Bex_def split: option.split)
+  apply (metis fun_sep_disj_1_fupdt(1) fun_split_1 sep_magma_1_right)
+   apply (metis fun_sep_disj_1_fupdt(1) fun_split_1 sep_magma_1_right)
+  apply auto
+
+lemma \<open>fun_upd 1 k o Some = (\<lambda>v. 1(k \<mapsto> v))\<close>
+  
 
 lemma
+  \<open>Transition_of' (\<phi>R_get_res_entry k F) ret \<subseteq> Id_on (P ret \<inter> SPACE)\<close>
+
+lemma
+  \<open> Transition_of' (\<phi>R_get_res_entry k F) ret = {(s,s').
+      (case get s k of Some v \<Rightarrow> (s,s') \<in> Transition_of' (F v) ret | _ \<Rightarrow> ret = Crash \<and> s \<in> SPACE)}\<close>
+  unfolding Transition_of'_def \<phi>R_get_res_def \<phi>R_get_res_entry_def
+  by (cases ret; clarsimp simp add: set_eq_iff split: option.split)
+
+lemma
+  \<open> Transition_of' (\<phi>R_get_res_entry k F) ret \<r>\<e>\<f>\<i>\<n>\<e>\<s> R ret \<w>.\<r>.\<t> basic_fiction \<close>
+
+
+
+lemma
+  \<open>pairself (\<lambda>x. 1(k := x)) ` {(Some any, u)} = {(1(k \<mapsto> any), 1(k := u))}\<close>
+  by (clarsimp simp add: set_eq_iff image_iff; blast)
+
+lemma "__updt_refinement__":
   \<open>{(x,y). x \<in> SPACE \<and> y = updt (\<lambda>f. f(k := u)) x}
-\<r>\<e>\<f>\<i>\<n>\<e>\<s> {(1(k \<mapsto> any)) | any. True} \<longrightarrow>\<^sub>R {(1(k := u))} \<w>.\<r>.\<t> basic_fiction \<i>\<n> {(1(k \<mapsto> any)) | any. True}\<close>
+\<r>\<e>\<f>\<i>\<n>\<e>\<s> {(1(k \<mapsto> any), 1(k := u))} \<w>.\<r>.\<t> basic_fiction \<i>\<n> {(1(k \<mapsto> any))}\<close>
   unfolding Fictional_Forward_Simulation_def
   apply (clarsimp simp add: basic_fiction_\<I> \<phi>expns prj.homo_mult times_fun_upd sep_disj_partial_map_upd
-        nonsepable_semigroup_sepdisj_fun)
-apply (clarsimp simp add: sep_disj_partial_map_upd
-          nonsepable_semigroup_sepdisj_fun mk_homo_mult)
-  subgoal premises prems for r R u' any
-  proof -
-    have [simp]: \<open>(get u' * (r * 1(k \<mapsto> any)))(k := u) = get u' * (r * 1(k := u))\<close>
-      by (metis domIff fun_upd_same fun_upd_upd mk_homo_mult option.distinct(1) prems(2) prems(4) sep_disj_get_name sep_disj_partial_map_upd)
-    have [simp]: \<open>get u' ## (r * 1(k := u))\<close>
-      by (metis mk_homo_mult nonsepable_semigroup_sepdisj_fun prems(2) prems(4) sep_disj_get_name sep_disj_multD1 sep_disj_multI1 sep_disj_multI2)
-    have [simp]: \<open>r ## 1(k := u)\<close>
-      by (meson nonsepable_semigroup_sepdisj_fun prems(2))
-    have [simp]: \<open>r ## (get u' * 1(k := u))\<close>
-      by (metis \<open>get u' ## r * 1(k := u)\<close> \<open>r ## 1(k := u)\<close> sep_disj_commuteI sep_disj_multI1 sep_mult_commute)
-    have [simp]: \<open>get u' ## 1(k := u)\<close>
-      using \<open>get u' ## r * 1(k := u)\<close> \<open>r ## 1(k := u)\<close> sep_disj_commute sep_disj_multD2 by blast
-    have \<open>clean u' * mk(get u') = u'\<close>
-      by (smt (verit, ccfv_threshold) fun_split_1 inj.homo_sep_wand mk_homo_mult prems(1) prems(2) prems(4) resource_kind.inj_prj_in_SPACE resource_kind_axioms sep_insertion.proj_inj sep_insertion_axioms sep_space_entry.sep_disj_mk_name sep_space_entry_axioms times_fupdt_1_apply_sep)
-    show ?thesis
-      apply (simp add: mk_homo_mult)
-      apply (rule exI[where x=u']; rule)
-      apply (smt (verit, best) \<open>clean u' * mk (get u') = u'\<close> \<open>get u' ## r * 1(k := u)\<close> \<open>r ## 1(k := u)\<close> mk_homo_mult sep_disj_clean sep_disj_mk sep_mult_assoc' sep_mult_left_commute)
-      by (metis \<open>clean u' * mk (get u') = u'\<close> \<open>get u' ## r * 1(k := u)\<close> \<open>r ## 1(k := u)\<close> mk_homo_mult prems(3) sep_disj_clean sep_disj_mk sep_disj_multI1)
-  qed
-  .
-      thm mk_homo_mult
-    apply (rule exI[where x=u']; simp add: prems)
-    apply rule
-     prefer 2
-  proof -
-    have t1[simp]: \<open>r ## 1(k := u)\<close>
-      by (meson nonsepable_semigroup_sepdisj_fun prems(1))
-    have t2: \<open>u' ## mk r * mk (1(k \<mapsto> any))\<close>
-      by (metis fun_1upd_homo inj.homo_mult prems(1) prems(3))
-    show \<open>u' ## mk (r * 1(k := u))\<close> 
-     apply (clarsimp simp add: mk_homo_mult)
-      thm mk_homo_mult
-      thm prems[simplified mk_homo_mult]
-
-  subgoal for r R u' any
-proof -
-    have t1: \<open>clean x * mk aa = x\<close>
-      by (metis fun_split_1 prems(8))
-    have t2: \<open>clean x ## (mk aa * mk (1(k := u)))\<close>
-      by (simp add: fun_1upd_homo)
-    show ?thesis
-      by (metis nonsepable_semigroup_sepdisj_fun prems(6) prems(9) sep_disj_mk sep_disj_multI1 sep_mult_assoc' t1 t2)
+        nonsepable_semigroup_sepdisj_fun SPACE_mult_homo \<r>_valid_split'
+        times_fun inj.homo_mult[symmetric] inject_wand_homo)
+  subgoal premises prems for r R u' a
+  proof (rule exI[where x=u']; simp add: prems; rule)
+    have [simp]: \<open>mk ((r * (a * 1(k \<mapsto> any)))(k := u)) = mk (r * (a * 1(k := u)))\<close>
+      by (smt (z3) domIff fun_split_1_not_dom fun_upd_same fun_upd_upd option.distinct(1) prems(3) prems(7) sep_disj_commuteI sep_disj_fun_nonsepable(1) sep_disj_multI1 sep_disj_partial_map_upd sep_mult_commute)
+    have t1[simp]: \<open>clean u' * mk a = u'\<close>
+      by (metis fun_split_1 prems(6))
+    show \<open>clean u' * mk ((r * (a * 1(k \<mapsto> any)))(k := u)) = u' * mk (r * 1(k := u))\<close>
+      apply simp
+      by (smt (verit, del_insts) fun_1upd_homo_right1 fun_upd_triv mk_homo_mult mult_1_class.mult_1_left nonsepable_semigroup_sepdisj_fun prems(3) prems(6) prems(7) sep_disj_multD1 sep_disj_multI1 sep_disj_multI2 sep_mult_left_commute)
+    show \<open>u' ## mk (r * 1(k := u))\<close>
+      by (smt (verit, del_insts) fun_upd_def inj.sep_disj_homo_semi nonsepable_semigroup_sepdisj_fun prems(3) prems(6) prems(7) sep_disj_fun_def sep_disj_multD1 sep_disj_multI1 sep_disj_multI2 sep_magma_1_left)
   qed .
-(*\<exists>ub. clean ua * mk ((get ua * (r * 1(k \<mapsto> any)))(k := u)) = ub * mk (r * 1(k := u)) \<and> ub \<in> R \<and> ub ## mk (r * 1(k := u))*)
-(*\<exists>xa. clean x * (mk a * mk (1(k := u))) = xa * mk (1(k := u)) \<and> xa \<in> R \<and> xa ## mk (1(k := u))*)
-  
-    apply rule
 
-  prefer 2
-  apply (meson nonsepable_semigroup_sepdisj_fun)
-  subgoal for x r R u'
-    apply (rule exI[where x=\<open>x(k:=u)\<close>])
-    
-thm sep_disj_partial_map_upd
 
-  unfolding \<phi>R_set_res_def Transition_of'_def
-  apply (cases evs; clarsimp simp add: \<phi>expns Fictional_Forward_Simulation_def basic_fiction_\<I>
-          prj.homo_mult)
+
+lemma transition_of_\<phi>R_set_res:
+  \<open>Transition_of' (\<phi>R_set_res (\<lambda>f. f(k := u))) ret = {(x,y). x \<in> SPACE \<and> y = updt (\<lambda>f. f(k := u)) x \<and> ret = Normal \<phi>V_none}\<close>
+  unfolding Transition_of'_def \<phi>R_set_res_def
+  by (cases ret; clarsimp simp add: set_eq_iff \<phi>V_none_def; rule; clarsimp)
+
+lemma transition_of_\<phi>R_set_res:
+  \<open>Transition_of' (\<phi>R_get_res (\<lambda>f. f(k := u))) ret = {(x,y). x \<in> SPACE \<and> y = updt (\<lambda>f. f(k := u)) x \<and> ret = Normal \<phi>V_none}\<close>
+  unfolding Transition_of'_def \<phi>R_set_res_def
+  by (cases ret; clarsimp simp add: set_eq_iff \<phi>V_none_def; rule; clarsimp)
+
 
 lemma
-  \<open>updt (\<lambda>f. f(k := u))\<close>
+  \<open>Transition_of' (\<phi>R_set_res (\<lambda>f. f(k := u))) ret
+  \<r>\<e>\<f>\<i>\<n>\<e>\<s> {(1(k \<mapsto> any), 1(k := u)) |any. True}
+  \<w>.\<r>.\<t> local.basic_fiction
+  \<i>\<n> {1(k \<mapsto> any) |any. True}\<close>
+  apply (subst transition_of_\<phi>R_set_res)
+  apply (rule refinement_sub_fun[OF "__updt_refinement__"])
+  by clarsimp
 
-term updt
-term Id
+
+end
+
+term \<open>(o) f\<close>
+
+term \<open>(o\<^sub>\<I>) I\<close>
+
+lemma
+  \<open>Id_on UNIV * Id_on {u} \<r>\<e>\<f>\<i>\<n>\<e>\<s> Id_on {f u} \<w>.\<r>.\<t> I \<i>\<n> {f u}\<close>
+  unfolding Fictional_Forward_Simulation_def
+  by (clarsimp simp add: Id_on_iff set_mult_expn Subjection_expn; blast)
+
+
+context cancl_perm_ins_homo begin
+
+lemma
+  \<open>Id_on UNIV * Id_on {u} \<r>\<e>\<f>\<i>\<n>\<e>\<s> {(share n (\<psi> u), share n (\<psi> u))} \<w>.\<r>.\<t> \<F>_functional \<psi> \<i>\<n> {share n (\<psi> u)}\<close>
+  for u :: \<open>'a::{sep_algebra, sep_cancel}\<close>
+  unfolding Fictional_Forward_Simulation_def
+  by (clarsimp simp add: Id_on_iff set_mult_expn Subjection_expn; blast)
+
+lemma
+  \<open>Id_on UNIV * {(u,v)} \<r>\<e>\<f>\<i>\<n>\<e>\<s> {(\<psi> u, \<psi> v)} \<w>.\<r>.\<t> \<F>_functional \<psi> \<i>\<n> {\<psi> u}\<close>
+  for u :: \<open>'a::{sep_algebra, sep_cancel}\<close>
+  unfolding Fictional_Forward_Simulation_def
+  apply (clarsimp simp add: Id_on_iff set_mult_expn Subjection_expn homo_sep_wand)
+  subgoal premises prems for R ru r1 r2
+  proof -
+    have t1: \<open>ru * u = (r1 * r2) * u\<close>
+      by (simp add: prems(1) prems(5) prems(6) sep_mult_assoc')
+    have t2: \<open>r1 * r2 ## u\<close>
+      using prems(5) prems(6) sep_disj_multI1 by blast
+    have t3: \<open>ru = r1 * r2\<close>
+      using prems(3) sep_cancel t1 t2 by blast
+    have t4: \<open>r2 ## v\<close>
+      using prems(4) prems(5) prems(6) sep_disj_multD1 sep_disj_multD2 t3 by blast
+    then have t5: \<open>\<psi> r2 ## \<psi> v\<close> by simp
+    show ?thesis
+      apply (simp add: t5)
+      apply (rule exI[where x=r1], rule exI[where x=\<open>r2 * v\<close>], simp add: t3)
+      by (metis local.homo_mult prems(2) prems(4) prems(5) prems(6) sep_disj_multD1 sep_disj_multI2 sep_mult_assoc t3 t4)
+  qed .
 
 end
 
