Phi_System/PhiSem_Formalization_Tools.thy
@@ -18,7 +18,7 @@ definition \<phi>M_assume :: \<open>bool \<Rightarrow> unit proc\<close>
 definition \<phi>M_getV_raw :: \<open>(VAL \<Rightarrow> 'v) \<Rightarrow> VAL \<phi>arg \<Rightarrow> ('v \<Rightarrow> 'y proc) \<Rightarrow> 'y proc\<close>
   where \<open>\<phi>M_getV_raw VDT_dest v F = F (VDT_dest (\<phi>arg.dest v))\<close>
 
-definition \<phi>M_getV :: \<open>TY \<Rightarrow> (VAL \<Rightarrow> 'v) \<Rightarrow> VAL \<phi>arg \<Rightarrow> ('v \<Rightarrow> 'y proc) \<Rightarrow> 'y::VALs proc\<close>
+definition \<phi>M_getV :: \<open>TY \<Rightarrow> (VAL \<Rightarrow> 'v) \<Rightarrow> VAL \<phi>arg \<Rightarrow> ('v \<Rightarrow> 'y proc) \<Rightarrow> 'y proc\<close>
   where \<open>\<phi>M_getV TY VDT_dest v F =
     (\<phi>M_assert (\<phi>arg.dest v \<in> Well_Type TY) \<ggreater> F (VDT_dest (\<phi>arg.dest v)))\<close>
 
@@ -112,10 +112,10 @@ definition \<phi>Res_Sat  :: \<open>resource \<Rightarrow> rassn \<Rightarrow> b
 abbreviation \<phi>Res_Sat'  :: \<open>resource \<Rightarrow> rassn \<Rightarrow> bool\<close> ("\<s>\<t>\<a>\<t>\<e> _ \<i>\<s> _" [11,11] 10)
   where \<open>\<phi>Res_Sat' s P \<equiv> \<phi>Res_Sat s (\<phi>Res_Spec P)\<close>
 
-definition \<phi>Comp_Sat :: \<open>'ret comp set \<Rightarrow> ('ret::VALs \<phi>arg \<Rightarrow> rassn) \<Rightarrow> (ABNM \<Rightarrow> rassn) \<Rightarrow> bool\<close>
+definition \<phi>Comp_Sat :: \<open>'ret comp set \<Rightarrow> ('ret \<phi>arg \<Rightarrow> rassn) \<Rightarrow> (ABNM \<Rightarrow> rassn) \<Rightarrow> bool\<close>
   where \<open>\<phi>Comp_Sat c S E \<longleftrightarrow> c \<subseteq> \<S> S E\<close>
 
-abbreviation \<phi>Comp_Sat' :: \<open>'ret comp set \<Rightarrow> ('ret::VALs \<phi>arg \<Rightarrow> rassn) \<Rightarrow> (ABNM \<Rightarrow> rassn) \<Rightarrow> bool\<close>
+abbreviation \<phi>Comp_Sat' :: \<open>'ret comp set \<Rightarrow> ('ret \<phi>arg \<Rightarrow> rassn) \<Rightarrow> (ABNM \<Rightarrow> rassn) \<Rightarrow> bool\<close>
                           ("_ \<r>\<e>\<s>\<u>\<l>\<t>\<s> \<i>\<n> _ \<t>\<h>\<r>\<o>\<w>\<s> _" [11,11,11] 10)
   where \<open>\<phi>Comp_Sat' c S E \<equiv> \<phi>Comp_Sat c (\<lambda>r. \<phi>Res_Spec (S r)) (\<lambda>e. \<phi>Res_Spec (E e))\<close>
 
@@ -1203,7 +1203,7 @@ lemma [\<phi>reason 1200 for \<open>?R \<heavy_comma> ?x \<Ztypecolon> Val ?raw 
 
 subsection \<open>Abnormal\<close>
 
-definition throw :: \<open>ABNM \<Rightarrow> 'ret::VALs proc\<close>
+definition throw :: \<open>ABNM \<Rightarrow> 'ret proc\<close>
   where \<open>throw raw = det_lift (Abnormal raw)\<close>
 
 lemma throw_reduce_tail[procedure_simps,simp]:
@@ -1212,7 +1212,7 @@ lemma throw_reduce_tail[procedure_simps,simp]:
 
 lemma "__throw_rule__"[intro!]:
   \<open> (\<And>a. X a \<i>\<m>\<p>\<l>\<i>\<e>\<s> X' a)
-\<Longrightarrow> \<p>\<r>\<o>\<c> (throw excep :: 'ret::VALs proc) \<lbrace> X excep \<longmapsto> Any \<rbrace> \<t>\<h>\<r>\<o>\<w>\<s> X'\<close>
+\<Longrightarrow> \<p>\<r>\<o>\<c> (throw excep :: 'ret proc) \<lbrace> X excep \<longmapsto> Any \<rbrace> \<t>\<h>\<r>\<o>\<w>\<s> X'\<close>
   unfolding \<phi>Procedure_def subset_iff det_lift_def throw_def Imply_def
   apply clarsimp
   by (meson Imply_def View_Shift_def view_shift_by_implication)
@@ -1224,7 +1224,7 @@ lemma throw_\<phi>app:
   apply clarsimp
   by (meson Imply_def View_Shift_def view_shift_by_implication)
 
-definition op_try :: "'ret proc \<Rightarrow> (ABNM \<Rightarrow> 'ret proc) \<Rightarrow> 'ret::VALs proc"
+definition op_try :: "'ret proc \<Rightarrow> (ABNM \<Rightarrow> 'ret proc) \<Rightarrow> 'ret proc"
   where \<open>op_try f g s = \<Union>((\<lambda>y. case y of Success x s' \<Rightarrow> {Success x s'}
                                        | Abnormal v s' \<Rightarrow> g v s'
                                        | AssumptionBroken \<Rightarrow> {AssumptionBroken}
@@ -1322,7 +1322,7 @@ subsubsection \<open>Legacy\<close>
 definition \<phi>M_get_res :: \<open>(resource \<Rightarrow> 'a) \<Rightarrow> ('a \<Rightarrow> 'ret proc) \<Rightarrow> 'ret proc\<close>
   where \<open>\<phi>M_get_res R F = (\<lambda>res. F (R res) res)\<close>
 
-definition \<phi>M_get_res_entry :: \<open>(resource \<Rightarrow> ('k \<rightharpoonup> 'a)) \<Rightarrow> 'k \<Rightarrow> ('a \<Rightarrow> 'ret proc) \<Rightarrow> 'ret::VALs proc\<close>
+definition \<phi>M_get_res_entry :: \<open>(resource \<Rightarrow> ('k \<rightharpoonup> 'a)) \<Rightarrow> 'k \<Rightarrow> ('a \<Rightarrow> 'ret proc) \<Rightarrow> 'ret proc\<close>
   where \<open>\<phi>M_get_res_entry R k F =
     \<phi>M_get_res R (\<lambda>res. case res k of Some v \<Rightarrow> F v | _ \<Rightarrow> (\<lambda>_. {Invalid}))\<close>
 
@@ -1344,7 +1344,7 @@ lemma (in resource) \<phi>R_get_res[intro!]:
 
 paragraph \<open>nonsepable_mono_resource\<close>
 
-definition (in nonsepable_mono_resource) \<phi>R_get_res_entry :: \<open>('T \<Rightarrow> 'ret proc) \<Rightarrow> 'ret::VALs proc\<close>
+definition (in nonsepable_mono_resource) \<phi>R_get_res_entry :: \<open>('T \<Rightarrow> 'ret proc) \<Rightarrow> 'ret proc\<close>
   where \<open>\<phi>R_get_res_entry F = \<phi>R_get_res (\<lambda>v. case v of Some v' \<Rightarrow> F (nosep.dest v')
                                                       | _ \<Rightarrow> (\<lambda>_. {Invalid}))\<close>
 
@@ -1357,7 +1357,7 @@ lemma (in nonsepable_mono_resource) \<phi>R_get_res_entry:
 paragraph \<open>partial_map_resource\<close>
 
 definition (in partial_map_resource)
-  \<phi>R_get_res_entry :: \<open>'key \<Rightarrow> ('val \<Rightarrow> 'ret proc) \<Rightarrow> 'ret::VALs proc\<close>
+  \<phi>R_get_res_entry :: \<open>'key \<Rightarrow> ('val \<Rightarrow> 'ret proc) \<Rightarrow> 'ret proc\<close>
   where \<open>\<phi>R_get_res_entry k F =
     \<phi>R_get_res (\<lambda>res. case res k of Some v \<Rightarrow> F v | _ \<Rightarrow> (\<lambda>_. {Invalid}))\<close>
 
@@ -1407,7 +1407,7 @@ end
 paragraph \<open>partial_map_resource2\<close>
 
 definition (in partial_map_resource2)
-    \<phi>R_get_res_entry :: \<open>'key \<Rightarrow> 'key2 \<Rightarrow> ('val \<Rightarrow> 'ret proc) \<Rightarrow> 'ret::VALs proc\<close>
+    \<phi>R_get_res_entry :: \<open>'key \<Rightarrow> 'key2 \<Rightarrow> ('val \<Rightarrow> 'ret proc) \<Rightarrow> 'ret proc\<close>
   where \<open>\<phi>R_get_res_entry k k2 F = \<phi>R_get_res (\<lambda>res.
     case res k k2 of Some v \<Rightarrow> F v | _ \<Rightarrow> (\<lambda>_. {Invalid}))\<close>
 
@@ -1596,7 +1596,7 @@ definition (in mapping_resource)
     \<phi>R_allocate_res_entry :: \<open>('key \<Rightarrow> bool)
                            \<Rightarrow> 'val
                            \<Rightarrow> ('key \<Rightarrow> 'ret proc)
-                           \<Rightarrow> 'ret::VALs proc\<close>
+                           \<Rightarrow> 'ret proc\<close>
   where \<open>\<phi>R_allocate_res_entry P init F =
     \<phi>R_get_res (\<lambda>res.
     let k = (@k. res k = 1 \<and> P k)
