Phi_Semantics/PhiSem_CF_Routine.thy
@@ -23,7 +23,7 @@ lemma "__routine__":
             \<t>\<h>\<r>\<o>\<w>\<s> (\<lambda>_. Brking_Frame label_ret Y))
       \<Longrightarrow> \<p>\<r>\<o>\<c> F label_ret (case_named (\<lambda>x. x) vs) \<lbrace> X (case_named id vs)\<heavy_comma> TECHNICAL Brk_Frame label_ret
                                           \<longmapsto> \<lambda>ret. Y ret\<heavy_comma> TECHNICAL Brk_Frame label_ret
-                                            \<rbrace> \<t>\<h>\<r>\<o>\<w>\<s> (\<lambda>e. \<^bold>b\<^bold>r\<^bold>e\<^bold>a\<^bold>k label_ret \<^bold>w\<^bold>i\<^bold>t\<^bold>h Y \<^bold>o\<^bold>r E e))
+                                            \<rbrace> \<t>\<h>\<r>\<o>\<w>\<s> (\<lambda>e. \<b>\<r>\<e>\<a>\<k> label_ret \<w>\<i>\<t>\<h> Y \<o>\<r> E e))
 \<Longrightarrow> \<p>\<r>\<o>\<c> op_routine TY_ARGs TY_RETs F vs \<lbrace> X vs \<longmapsto> Y \<rbrace> \<t>\<h>\<r>\<o>\<w>\<s> E\<close>
   unfolding op_routine_def
   \<medium_left_bracket> premises [\<phi>reason 5000] and [\<phi>reason 5000] and _ and F
